thys/Flyspeck-Tame/Maps.thy
@@ -4,13 +4,13 @@ begin
 
 locale maps =
 fixes empty :: "'m"
-and up :: "'m \<Rightarrow> 'a \<Rightarrow> 'b list \<Rightarrow> 'm"
+and up :: "'a \<Rightarrow> 'b list \<Rightarrow> 'm \<Rightarrow> 'm"
 and map_of :: "'m \<Rightarrow> 'a \<Rightarrow> 'b list"
 and M :: "'m \<Rightarrow> bool"
 assumes map_empty: "map_of empty = (%a. [])"
-and map_up: "map_of (up m a b) = (map_of m)(a := b)"
+and map_up: "map_of (up a b m) = (map_of m)(a := b)"
 and M_empty: "M empty"
-and M_up: "M m \<Longrightarrow> M (up m a b)"
+and M_up: "M m \<Longrightarrow> M (up a b m)"
 begin
 
 definition "set_of m = (UN x. set(map_of m x))"
@@ -19,7 +19,7 @@ end
 
 locale set_mod_maps = maps empty up map_of M + quasi_order qle
 for empty :: "'m"
-and up :: "'m \<Rightarrow> 'a \<Rightarrow> 'b list \<Rightarrow> 'm"
+and up :: "'a \<Rightarrow> 'b list \<Rightarrow> 'm \<Rightarrow> 'm"
 and map_of :: "'m \<Rightarrow> 'a \<Rightarrow> 'b list"
 and M :: "'m \<Rightarrow> bool"
 and qle :: "'b \<Rightarrow> 'b \<Rightarrow> bool" (infix "\<preceq>" 60)
@@ -33,7 +33,7 @@ begin
 
 definition "insert_mod x m =
   (let k = key x; ys = map_of m k
-   in if (EX y : set ys. subsumed x y) then m else up m k (x#ys))"
+   in if (EX y : set ys. subsumed x y) then m else up k (x#ys) m)"
 
 end
 
