thys/Flyspeck-Tame/ArchCompProps.thy
@@ -21,90 +21,65 @@ by(simp add:pre_iso_test_def iso_correct inj_on_rotate_min_iff[symmetric]
             distinct_map nof_vertices_def length_remdups_concat)
 
 lemma trie_all_eq_set_of_trie:
-  "Tries.inv t \<Longrightarrow> Tries.all P t = (\<forall>v \<in> Tries.set_of t. P v)"
-apply(induct t rule:Tries.inv.induct)
-apply (auto simp: Tries.set_of_def)
-  apply(case_tac a)
-   apply simp
-  apply auto
-  apply blast
- apply(erule allE)
- apply(erule impE)
-  apply(rule_tac x = "[]" in exI)
-  apply(rule HOL.refl)
- apply simp
-apply(erule meta_allE)+
-apply(erule meta_impE)
- apply assumption
-apply(erule meta_impE)
- apply fast
-apply(erule meta_impE)
- apply fast
-apply clarsimp
-apply(erule allE)
-apply(erule impE)
- apply(rule_tac x = "a#aa" in exI)
-apply(rule HOL.refl)
-apply auto
-done
-
+  "invar_trie t \<Longrightarrow> all_trie (list_all P) t = (\<forall>v \<in> set_tries t. P v)"
+by(simp add: all_trie_eq_ran set_tries_eq_ran)
 
 lemma samet_imp_iso_seteq:
-assumes pre1: "\<And>gs g. gsopt = Some gs \<Longrightarrow> g \<in> Tries.set_of gs \<Longrightarrow> pre_iso_test g"
+assumes pre1: "\<And>gs g. gsopt = Some gs \<Longrightarrow> g \<in> set_tries gs \<Longrightarrow> pre_iso_test g"
 and pre2: "\<And>g. g \<in> set arch \<Longrightarrow> pre_iso_test g"
-and inv: "!!gs. gsopt = Some gs \<Longrightarrow> Tries.inv gs"
+and inv: "!!gs. gsopt = Some gs \<Longrightarrow> invar_trie gs"
 and same: "samet gsopt arch"
-shows "\<exists>gs. gsopt = Some gs \<and> Tries.set_of gs =\<^sub>\<simeq> set arch"
+shows "\<exists>gs. gsopt = Some gs \<and> set_tries gs =\<^sub>\<simeq> set arch"
 proof -
-  obtain gs where [simp]: "gsopt = Some gs" and test1: "\<And>g. g \<in> Tries.set_of gs \<Longrightarrow>
+  obtain gs where [simp]: "gsopt = Some gs" and test1: "\<And>g. g \<in> set_tries gs \<Longrightarrow>
     \<exists>h \<in> set arch. iso_test g h" and test2: "\<And>g. g \<in> set arch \<Longrightarrow>
-    \<exists>h \<in> Tries.set_of gs. iso_test g h"
+    \<exists>h \<in> set_tries gs. iso_test g h"
     using same inv
-    by(force simp: samet_def trie_all_eq_set_of_trie inv_of_list
+    by(force simp: samet_def trie_all_eq_set_of_trie invar_of_list all_tries_def
       split:option.splits
-      dest: in_set_lookup_of_listD in_set_lookup_set_ofD)
-  have "Tries.set_of gs \<subseteq>\<^sub>\<simeq> set arch"
+      dest: in_set_lookup_of_listD in_set_lookup_set_triesD)
+  have "set_tries gs \<subseteq>\<^sub>\<simeq> set arch"
   proof (auto simp:qle_gr.defs)
-    fix g assume g: "g \<in> Tries.set_of gs"
+    fix g assume g: "g \<in> set_tries gs"
     obtain h where h: "h \<in> set arch" and test: "iso_test g h"
       using test1[OF g] by blast
     thus "\<exists>h\<in>set arch. g \<simeq> h"
       using h pre1[OF _ g] pre2[OF h] by (auto simp:iso_test_correct)
   qed
   moreover
-  have "set arch \<subseteq>\<^sub>\<simeq> Tries.set_of gs"
+  have "set arch \<subseteq>\<^sub>\<simeq> set_tries gs"
   proof (auto simp:qle_gr.defs)
     fix g assume g: "g \<in> set arch"
-    obtain h where h: "h \<in> Tries.set_of gs" and test: "iso_test g h"
+    obtain h where h: "h \<in> set_tries gs" and test: "iso_test g h"
       using test2[OF g] by blast
-    thus "\<exists>h \<in> Tries.set_of gs. g \<simeq> h"
+    thus "\<exists>h \<in> set_tries gs. g \<simeq> h"
       using h pre1[OF _ h] pre2[OF g] by (auto simp:iso_test_correct)
   qed
   ultimately show ?thesis by (auto simp: qle_gr.seteq_qle_def)
 qed
 
 lemma samet_imp_iso_subseteq:
-assumes pre1: "\<And>gs g. gsopt = Some gs \<Longrightarrow> g \<in> Tries.set_of gs \<Longrightarrow> pre_iso_test g"
+assumes pre1: "\<And>gs g. gsopt = Some gs \<Longrightarrow> g \<in> set_tries gs \<Longrightarrow> pre_iso_test g"
 and pre2: "\<And>g. g \<in> set arch \<Longrightarrow> pre_iso_test g"
-and inv: "!!gs. gsopt = Some gs \<Longrightarrow> Tries.inv gs"
+and inv: "!!gs. gsopt = Some gs \<Longrightarrow> invar_trie gs"
 and same: "samet gsopt arch"
-shows "\<exists>gs. gsopt = Some gs \<and> Tries.set_of gs \<subseteq>\<^sub>\<simeq> set arch"
+shows "\<exists>gs. gsopt = Some gs \<and> set_tries gs \<subseteq>\<^sub>\<simeq> set arch"
 using qle_gr.seteq_qle_def assms samet_imp_iso_seteq by metis
 
 definition [code del]:
-"insert_mod_trie = set_mod_maps.insert_mod Tries.update Tries.lookup iso_test hash"
+"insert_mod_trie = set_mod_maps.insert_mod update_trie lookup_tries iso_test hash"
 definition [code del]:
-"worklist_tree_coll_trie = set_modulo.worklist_tree_coll (Tries [] []) insert_mod_trie"
+"worklist_tree_coll_trie = set_modulo.worklist_tree_coll (Trie None []) insert_mod_trie"
 definition [code del]:
 "worklist_tree_coll_aux_trie = set_modulo.worklist_tree_coll_aux insert_mod_trie"
 definition [code del]:
 "insert_mod2_trie = set_modulo.insert_mod2 insert_mod_trie"
 
 interpretation set_mod_trie:
-  set_mod_maps "Tries [] []" Tries.update Tries.lookup Tries.inv "op \<simeq>" iso_test pre_iso_test hash
-where "set_modulo.worklist_tree_coll (Tries [] []) insert_mod_trie = worklist_tree_coll_trie"
+  set_mod_maps "Trie None []" update_trie lookup_tries invar_trie "op \<simeq>" iso_test pre_iso_test hash
+where "set_modulo.worklist_tree_coll (Trie None []) insert_mod_trie = worklist_tree_coll_trie"
 and "set_modulo.worklist_tree_coll_aux insert_mod_trie = worklist_tree_coll_aux_trie"
-and "set_mod_maps.insert_mod Tries.update Tries.lookup iso_test hash = insert_mod_trie"
+and "set_mod_maps.insert_mod update_trie lookup_tries iso_test hash = insert_mod_trie"
 and "set_modulo.insert_mod2 insert_mod_trie = insert_mod2_trie"
 proof unfold_locales
 qed (auto simp:iso_test_correct worklist_tree_coll_trie_def worklist_tree_coll_aux_trie_def insert_mod_trie_def insert_mod2_trie_def)
@@ -118,28 +93,28 @@ definition tameEnumFilter :: "nat \<Rightarrow> (nat,nat fgraph)tries option" wh
 "tameEnumFilter p = enum_filter_finals (next_tame p) [Seed p]"
 
 lemma TameEnum_tameEnumFilter:
-  "tameEnumFilter p = Some t \<Longrightarrow>  Tries.set_of t  =\<^sub>\<simeq> fgraph ` TameEnum\<^bsub>p\<^esub>"
+  "tameEnumFilter p = Some t \<Longrightarrow>  set_tries t  =\<^sub>\<simeq> fgraph ` TameEnum\<^bsub>p\<^esub>"
 apply(auto simp: tameEnumFilter_def TameEnumP_def enum_filter_finals_def)
 apply(drule set_mod_trie.worklist_tree_coll_equiv[OF _ inv_inv_next_tame])
-apply (auto simp: Tries.set_of_conv inv_Seed mgp_pre_iso_test RTranCl_conv)
+apply (auto simp: set_of_conv inv_Seed mgp_pre_iso_test RTranCl_conv)
 done
 
 lemma tameEnumFilter_subseteq_TameEnum:
-  "tameEnumFilter p = Some t \<Longrightarrow> Tries.set_of t <= fgraph ` TameEnum\<^bsub>p\<^esub>"
+  "tameEnumFilter p = Some t \<Longrightarrow> set_tries t <= fgraph ` TameEnum\<^bsub>p\<^esub>"
 by(auto simp add:tameEnumFilter_def TameEnumP_def enum_filter_finals_def
-     Tries.set_of_conv inv_Seed mgp_pre_iso_test RTranCl_conv
+     set_of_conv inv_Seed mgp_pre_iso_test RTranCl_conv
      dest!: set_mod_trie.worklist_tree_coll_subseteq[OF _ inv_inv_next_tame])
 
 
 lemma inv_tries_tameEnumFilter:
-  "tameEnumFilter p = Some t \<Longrightarrow> Tries.inv t"
+  "tameEnumFilter p = Some t \<Longrightarrow> invar_trie t"
 unfolding tameEnumFilter_def enum_filter_finals_def
 by(erule set_mod_trie.worklist_tree_coll_inv)
 
 theorem combine_evals_filter:
  "\<forall>g \<in> set arch. pre_iso_test g \<Longrightarrow> samet (tameEnumFilter p) arch
   \<Longrightarrow> fgraph ` TameEnum\<^bsub>p\<^esub> \<subseteq>\<^sub>\<simeq> set arch"
-apply(subgoal_tac "\<exists>t. tameEnumFilter p = Some t \<and> Tries.set_of t \<subseteq>\<^sub>\<simeq> set arch")
+apply(subgoal_tac "\<exists>t. tameEnumFilter p = Some t \<and> set_tries t \<subseteq>\<^sub>\<simeq> set arch")
  apply(metis TameEnum_tameEnumFilter qle_gr.seteq_qle_def qle_gr.subseteq_qle_trans)
 apply(fastforce intro!: samet_imp_iso_subseteq
   dest: inv_tries_tameEnumFilter tameEnumFilter_subseteq_TameEnum mgp_TameEnum mgp_pre_iso_test)
